removed some addr_in_page, lending WIP

theories/proofmode.v
@@ -12,14 +12,17 @@ Class FramableRegisterPointsto `{HypervisorConstants} (r: reg_name) (i: VMID) (w
 Class FramableMemoryPointsto (a: Addr) (w: Addr) := {}.
 #[export] Hint Mode FramableMemoryPointsto + - : typeclass_instances.
 
-Class FramableAccessPointsto `{HypervisorConstants} (i: VMID) (s: gset PID) := {}.
-#[export] Hint Mode FramableAccessPointsto + + - : typeclass_instances.
+Class FramablePageTablePointsto `{HypervisorConstants} (i: VMID) (s: gset PID) := {}.
+#[export] Hint Mode FramablePageTablePointsto + + - : typeclass_instances.
 
 Class FramableTXPointsto `{HypervisorConstants} (i: VMID) (p: PID) := {}.
 #[export] Hint Mode FramableTXPointsto + + - : typeclass_instances.
 
 Class FramableRXPointsto `{HypervisorConstants} (i: VMID) (p: PID) := {}.
 #[export] Hint Mode FramableRXPointsto + + - : typeclass_instances.
+
+Class FramableHandlePool (s: gset handle) := {}.
+#[export] Hint Mode FramableHandlePool - : typeclass_instances.
 
 Instance FramableRegisterPointsto_default `{HypervisorConstants} r i w :
   FramableRegisterPointsto r i w
@@ -29,8 +32,8 @@ Instance FramableMemoryPointsto_default a w :
   FramableMemoryPointsto a w
 | 100. Qed.
 
-Instance FramableAccessPointsto_default `{HypervisorConstants} i s :
-  FramableAccessPointsto i s
+Instance FramablePageTablePointsto_default `{HypervisorConstants} i s :
+  FramablePageTablePointsto i s
 | 100. Qed.
 
 Instance FramableTXPointsto_default `{HypervisorConstants} i p :
@@ -51,9 +54,19 @@ Instance FramableMachineResource_mem `{gen_VMG Σ} a w :
   FramableMachineResource (a ->a w).
 Qed.
 
+Instance FramableMachineResource_own `{gen_VMG Σ} i q s :
+  FramablePageTablePointsto i s →
+  FramableMachineResource (O@i :={q}[s]).
+Qed.
+
 Instance FramableMachineResource_access `{gen_VMG Σ} i q s :
-  FramableAccessPointsto i s →
+  FramablePageTablePointsto i s →
   FramableMachineResource (A@i :={q}[s]).
+Qed.
+
+Instance FramableMachineResource_excl `{gen_VMG Σ} i q s :
+  FramablePageTablePointsto i s →
+  FramableMachineResource (E@i :={q}[s]).
 Qed.
 
 Instance FramableMachineResource_TX `{gen_VMG Σ} i p :
@@ -64,4 +77,9 @@ Qed.
 Instance FramableMachineResource_RX `{gen_VMG Σ} i p :
   FramableRXPointsto i p →
   FramableMachineResource (RX@i := p).
+Qed.
+
+Instance FramableMachineResource_hp`{gen_VMG Σ} q s :
+  FramableHandlePool s →
+  FramableMachineResource (hp{q}[s]).
 Qed.
